ttcan: convert to autolift

example/ttcan/Network.TTCan.Impl.Triggers.fst
@@ -12,11 +12,12 @@ module SugarBase = Pipit.Sugar.Base
 module SugarTac  = Pipit.Sugar.Shallow.Tactics
 
 open Pipit.Sugar.Shallow.Tactics.Lift
-module Cse = Pipit.Tactics.Cse
 
 module UInt8 = FStar.UInt8
 module UInt64= FStar.UInt64
 module Cast  = FStar.Int.Cast
+
+module Tac = FStar.Tactics
 
 (***** Non-streaming helper functions ****)
 let trigger_check_enabled (cycle_index: cycle_index) (trigger: trigger): bool =
@@ -26,70 +27,106 @@ let trigger_check_enabled (cycle_index: cycle_index) (trigger: trigger): bool =
   let offset8 = S32R.s32r_to_u8 trigger.cycle_offset in
   UInt8.logand mask8 index8 = offset8
 
-let trigger_compute_expiry (cfg: config) (ix: trigger_index) (trigger: trigger): ntu =
+let trigger_tx_ref_expiry (cfg: config) (ix: trigger_index) (trigger: trigger): ntu =
   let open UInt64 in
   let tm = S32R.s32r_to_u64 trigger.time_mark in
-  (* We keep trying to send Tx_Ref_Triggers until they're pre-empted by the next trigger, so their expiry is very large.
-    We keep trying to send Tx_Triggers for Tx_Enable_Window ntus.
-    We don't need to keep trying Rx_Triggers or Watch_Triggers. *)
-  match trigger.trigger_type with
-  | Tx_Ref_Trigger ->
-    tm +^ 65535uL
-  | Tx_Trigger ->
-    tm +^ S32R.s32r_to_u64 cfg.tx_enable_window
-  | _ ->
-    tm
+  tm +^ S32R.s32r_to_u64 cfg.tx_enable_window
+
+let trigger_offset (ref_trigger_offset: ref_offset) (tr: trigger): trigger =
+  let time_mark =
+    match tr.trigger_type with
+    | Tx_Ref_Trigger ->
+      // use saturating addition to clamp to [0,65535]
+      S32R.add_sat tr.time_mark ref_trigger_offset
+    | _ ->
+      tr.time_mark
+  in
+  { tr with time_mark }
 
 
 let trigger_load (cfg: config) (ix: trigger_index) (ref_trigger_offset: ref_offset): trigger =
   [@@no_inline_let] // do not inline index function into use-sites
-  let base = cfg.trigger_index_fun ix in
-  let time_mark =
-    match base.trigger_type with
-    | Tx_Ref_Trigger ->
-      // use saturating addition to clamp to [0,65535]
-      S32R.add_sat base.time_mark ref_trigger_offset
-    | _ ->
-      base.time_mark
-  in
-  { base with time_mark }
+  let base = cfg.triggers.trigger_index_fun ix in
+  trigger_offset ref_trigger_offset base
+
+(* Specification-only - compute next active.
+  This must not be called as executable code, as it would have the wrong
+  complexity (linear in the number of triggers, rather than constant).
+  Mark it as noextract so it can't be extracted. Really it should be ghost,
+  but Pipit doesn't support ghost code yet.
+  *)
+noextract
+let rec active_next_after_index (triggers: triggers) (cycle_index: cycle_index) (time: nat) (index: nat)
+  : Tot
+    (n: nat { 0 <= n /\ n <= S32R.v triggers.trigger_count })
+    (decreases (S32R.v triggers.trigger_count - index)) =
+  if index >= S32R.v triggers.trigger_count
+  then S32R.v triggers.trigger_count
+  else
+    let tr = triggers.trigger_index_fun (S32R.s32r index) in
+    if S32R.v tr.time_mark > time && trigger_check_enabled cycle_index tr
+    then index
+    else active_next_after_index triggers cycle_index time (index + 1)
+
+noextract
+let active_next_after (triggers: triggers) (cycle_index: cycle_index) (time: nat)
+  : (n: nat { 0 <= n /\ n <= S32R.v triggers.trigger_count }) =
+  active_next_after_index triggers cycle_index time 0
+
+noextract
+let rec active_now_index (triggers: triggers) (cycle_index: cycle_index) (time: nat) (index: nat { index < S32R.v triggers.trigger_count })
+  : Tot
+    (n: nat { 0 <= n /\ n <= S32R.v triggers.trigger_count })
+    (decreases index) =
+  if index = 0
+  then 0
+  else
+    let tr = triggers.trigger_index_fun (S32R.s32r index) in
+    if S32R.v tr.time_mark <= time && trigger_check_enabled cycle_index tr
+    then index
+    else active_now_index triggers cycle_index time (index - 1)
+
+noextract
+let active_now (triggers: triggers) (cycle_index: cycle_index) (time: nat)
+  : (n: nat { 0 <= n /\ n <= S32R.v triggers.trigger_count }) =
+  active_now_index triggers cycle_index time (S32R.v triggers.trigger_count - 1)
 
 (* Result of pre-fetch node *)
 type prefetch_result = {
   index:   trigger_index;
   // True when trigger is enabled in current basic cycle index
   enabled: bool;
-  // Trigger end time: when to give up trying for triggers with retries (Tx_Message and Tx_Ref_Message)
-  expiry:  ntu;
-  // Trigger information
-  trigger: trigger;
+  // Updated time (after ref-trigger-offset applied to tx-ref triggers)
+  time_mark: ntu_config;
 }
 
 type fetch_result = {
   current:    prefetch_result;
   // True when trigger changes
   is_new:     bool;
-  // True if trigger's start time <= now
+  // True if trigger has started or is about to start.
+  // trigger's post-ref-trigger-offset start time <= now + ttcan_exec_period
   is_started: bool;
-  // True if trigger's end time <= now
-  is_expired: bool;
-  // Total enabled and disabled triggers seen this cycle
-  tx_count:   trigger_count;
+  // Actual trigger with type, message id etc. time-mark and cycle indices aren't needed here
+  trigger: trigger;
 }
 
 
 (**** Streaming instances for records ****)
 instance has_stream_prefetch_result: S.has_stream prefetch_result = {
   ty_id       = [`%prefetch_result];
-  val_default = { enabled = S.val_default; index = S.val_default; expiry = S.val_default; trigger = S.val_default; };
+  val_default = { enabled = S.val_default; index = S.val_default; time_mark = S.val_default; };
 }
 
 instance has_stream_fetch_result: S.has_stream fetch_result = {
   ty_id       = [`%fetch_result];
-  val_default = { current = S.val_default; is_new = S.val_default;  is_started = S.val_default; is_expired = S.val_default; tx_count = S.val_default; };
+  val_default = { current = S.val_default; is_new = S.val_default;  is_started = S.val_default; trigger = S.val_default; };
 }
 
-#push-options "--ext pipit:lift:debug"
+let trigger_delay (cycle_time: ntu) (fetch: fetch_result): ntu =
+  if fetch.is_started
+  then 0uL
+  else U64.(cycle_time - S32R.s32r_to_u64 fetch.trigger.time_mark)
 
 (*
   Pre-fetch the next enabled trigger.
@@ -104,7 +141,6 @@ instance has_stream_fetch_result: S.has_stream fetch_result = {
 
   Invariant: all trigger entries before trigger_index have start time in the past or are not enabled this cycle.
 *)
-// [@@FStar.Tactics.preprocess_with Pipit.Tactics.Cse.cse]
 let prefetch
   (cfg: config)
   (reset_ck:           stream bool)
@@ -115,7 +151,7 @@ let prefetch
     : stream prefetch_result #_ =
   rec' (fun fetch ->
     let pre_index = (S32R.s32r 0 <: trigger_index) `fby` fetch.index in
-    let advance = false `fby` (not fetch.enabled || U64.(S32R.s32r_to_u64 fetch.trigger.time_mark <= cycle_time)) in
+    let advance = false `fby` (not fetch.enabled || U64.(S32R.s32r_to_u64 fetch.time_mark <= cycle_time)) in
     let index =
       if reset_ck
       then S32R.s32r 0
@@ -124,38 +160,40 @@ let prefetch
       else pre_index in
     let trigger = trigger_load cfg index ref_trigger_offset in
     let enabled = trigger_check_enabled cycle_index trigger in
-    let expiry  = trigger_compute_expiry cfg index trigger in
-    { index; enabled; expiry; trigger })
+    { index; enabled; time_mark = trigger.time_mark })
 
 %splice[prefetch_core] (autolift_binds [`%prefetch])
 
+
+// TODO: move to tx controller;
+// this should only reset when reference message cycle = 0
 (*^5.1 Tx_Count: each time a Tx_Trigger becomes active, Tx_Count is incremented. Tx_Count is not incremented beyond Expected_Tx_Trigger. *)
 (* CLARIFICATION: the definition of "active" is not entirely clear to me.
   Is it whenever a Tx_Trigger trigger array entry is encountered by the trigger loop, or is it only when the trigger is enabled for the current cycle index?
   I think it must be every time it's encountered by the loop, because otherwise we would underflow for a periodic trigger that doesn't transmit every cycle.
   *)
-let tx_counter
-  (reset_ck: stream bool)
-  (prefetch: stream prefetch_result #_)
-    : stream trigger_count #_ =
-  let open S32R in
-  rec' (fun tx_count ->
-    let prev: trigger_count =
-      if reset_ck
-      then s32r 0
-      else s32r 0 `fby` tx_count in
-    let incr =
-      Util.edge #trigger_index prefetch.index &&
-      prefetch.trigger.trigger_type = Tx_Trigger in
-    if incr
-    then inc_sat prev
-    else prev)
-
-%splice[tx_counter_core] (autolift_binds [`%tx_counter])
+// let tx_counter
+//   (reset_ck: stream bool)
+//   (prefetch: stream prefetch_result #_)
+//     : stream trigger_count #_ =
+//   let open S32R in
+//   rec' (fun tx_count ->
+//     let prev: trigger_count =
+//       if reset_ck
+//       then s32r 0
+//       else s32r 0 `fby` tx_count in
+//     let incr =
+//       Util.edge #trigger_index prefetch.index &&
+//       prefetch.trigger.trigger_type = Tx_Trigger in
+//     if incr
+//     then inc_sat prev
+//     else prev)
+// %splice[tx_counter_core] (autolift_binds [`%tx_counter])
 
 (*
   Fetch the current trigger, or the next one if there is no current trigger.
 *)
+[@@Tac.preprocess_with preprocess]
 let fetch
   (cfg: config)
   (reset_ck:    stream bool)
@@ -163,26 +201,16 @@ let fetch
   (cycle_index: stream cycle_index #_)
   (ref_trigger_offset: stream ref_offset #_)
     : stream fetch_result #_ =
-  let is_trigger_started (tr: stream trigger #_): stream bool =
-    U64.(S32R.s32r_to_u64 tr.time_mark <= cycle_time) in
-  let next = prefetch cfg reset_ck cycle_time cycle_index ref_trigger_offset in
-  rec' (fun (fetch: stream fetch_result #_) ->
-    // If the new trigger is enabled and is ready to start, then the new trigger has precedence. This case allows Watch_Triggers to pre-empt Tx_Ref_Triggers, as Tx_Ref_Triggers do not expire otherwise.
-    // Otherwise, if the old trigger expired on the previous tick, then we the new trigger can be started. The delay here ensures that the caller gets a chance to handle the expired triggers.
-    let advance = reset_ck ||
-      (next.enabled && is_trigger_started next.trigger) ||
-      (false `fby` fetch.is_expired)
-    in
-    let current =
-      next ->^ (if advance then next else pre fetch.current)
-    in
-
-    let index = current.index in
-    let is_new = Util.edge #trigger_index index in
-    let is_started = is_trigger_started current.trigger in
-    let is_expired = U64.(current.expiry <= cycle_time) in
-    let tx_count = tx_counter reset_ck next in
-    { current; is_new; is_started; is_expired; tx_count; }
-  )
+  let is_trigger_starting (time_mark: stream ntu_config #_): stream bool =
+    U64.(S32R.s32r_to_u64 time_mark <= cycle_time) in
+  let next      = prefetch cfg reset_ck cycle_time cycle_index ref_trigger_offset in
+  let take_next = reset_ck || (next.enabled && is_trigger_starting next.time_mark) in
+  let rec current =
+    next ->^ (if take_next then next else pre current)
+  in
+  let is_new = Util.edge #trigger_index current.index in
+  let is_started = is_trigger_starting current.time_mark in
+  let trigger = trigger_load cfg current.index ref_trigger_offset in
+  { current; is_new; is_started; trigger; }
 
 %splice[fetch_core] (autolift_binds [`%fetch])
